<?xml version="1.0"?>


<!DOCTYPE rdf:RDF [
    <!ENTITY motifs "http://purl.org/net/wf-motifs#" >
    <!ENTITY owl "http://www.w3.org/2002/07/owl#" >
    <!ENTITY xsd "http://www.w3.org/2001/XMLSchema#" >
    <!ENTITY rdfs "http://www.w3.org/2000/01/rdf-schema#" >
    <!ENTITY rdf "http://www.w3.org/1999/02/22-rdf-syntax-ns#" >
]>


<rdf:RDF xmlns="http://purl.org/net/wf-motifs#"
     xml:base="http://purl.org/net/wf-motifs"
     xmlns:rdfs="http://www.w3.org/2000/01/rdf-schema#"
     xmlns:owl="http://www.w3.org/2002/07/owl#"
     xmlns:xsd="http://www.w3.org/2001/XMLSchema#"
     xmlns:rdf="http://www.w3.org/1999/02/22-rdf-syntax-ns#"
     xmlns:motifs="http://purl.org/net/wf-motifs#">
    <owl:Ontology rdf:about="http://purl.org/net/wf-motifs">
        <rdfs:label xml:lang="en">Workflow Motif Ontology</rdfs:label>
        <rdfs:comment>This ontology is based on the paper: Common Motifs in Scientific Workflows:An Empirical Analysis, by Daniel Garijo, Pinar Alper, Khalid Belhajjame, Oscar Corcho, Yolanda Gil and Carole Goble</rdfs:comment>
        <owl:versionInfo>Version 1.01</owl:versionInfo>
        <rdfs:comment xml:lang="en">Workflow Motif Ontology, created by Daniel Garijo, Pinar Alper and Khalid Belhajjame</rdfs:comment>
    </owl:Ontology>
    


    <!-- 
    ///////////////////////////////////////////////////////////////////////////////////////
    //
    // Annotation properties
    //
    ///////////////////////////////////////////////////////////////////////////////////////
     -->

    


    <!-- 
    ///////////////////////////////////////////////////////////////////////////////////////
    //
    // Datatypes
    //
    ///////////////////////////////////////////////////////////////////////////////////////
     -->

    


    <!-- 
    ///////////////////////////////////////////////////////////////////////////////////////
    //
    // Object Properties
    //
    ///////////////////////////////////////////////////////////////////////////////////////
     -->

    


    <!-- http://purl.org/net/wf-motifs#implementsMotif -->

    <owl:ObjectProperty rdf:about="&motifs;implementsMotif">
        <rdfs:label xml:lang="en">implements motif</rdfs:label>
        <rdfs:comment>This object property is used to annotate a step in the workflow, a group of steps, a subworkflow, or a workflow with a motif.</rdfs:comment>
        <rdfs:range rdf:resource="&motifs;Motif"/>
    </owl:ObjectProperty>
    


    <!-- http://purl.org/net/wf-motifs#implementsOperationMotif -->

    <owl:ObjectProperty rdf:about="&motifs;implementsOperationMotif">
        <rdfs:label xml:lang="en">implements operation motif</rdfs:label>
        <rdfs:comment xml:lang="en">Object property that connects a, workflow step with its correspondent OperationMotif.</rdfs:comment>
        <rdfs:range rdf:resource="&motifs;OperationMotif"/>
        <rdfs:subPropertyOf rdf:resource="&motifs;implementsMotif"/>
    </owl:ObjectProperty>
    


    <!-- http://purl.org/net/wf-motifs#implementsWorkflowMotif -->

    <owl:ObjectProperty rdf:about="&motifs;implementsWorkflowMotif">
        <rdfs:label xml:lang="en">implements workflow motif</rdfs:label>
        <rdfs:comment xml:lang="en">Object property that relates a Workflow to its correspondent motif</rdfs:comment>
        <rdfs:range rdf:resource="&motifs;WorkflowMotif"/>
        <rdfs:subPropertyOf rdf:resource="&motifs;implementsMotif"/>
    </owl:ObjectProperty>
    


    <!-- 
    ///////////////////////////////////////////////////////////////////////////////////////
    //
    // Classes
    //
    ///////////////////////////////////////////////////////////////////////////////////////
     -->

    


    <!-- http://purl.org/net/wf-motifs#AsynchronousInvocation -->

    <owl:Class rdf:about="&motifs;AsynchronousInvocation">
        <rdfs:label xml:lang="en">Asynchronous invocation</rdfs:label>
        <rdfs:subClassOf rdf:resource="&motifs;IntraWorkflowMotif"/>
        <rdfs:comment xml:lang="en">Certain activities such as analysis or visualizations could be performed through interaction with stateful (web) services that allow for creation of jobs over remote grid environments. These are typically performed via invocation of multiple operations at a service endpoint. </rdfs:comment>
    </owl:Class>
    


    <!-- http://purl.org/net/wf-motifs#AtomicWorkflow -->

    <owl:Class rdf:about="&motifs;AtomicWorkflow">
        <rdfs:label xml:lang="en">Atomic workflow</rdfs:label>
        <rdfs:subClassOf rdf:resource="&motifs;InterWorkflowMotif"/>
        <rdfs:comment>Motif used to characetrize the workflows that perform an atomic unit of functionality, which effectively requires no sub-workflow usage. Typically these workflows are designed to be included in other work- flows. Atomic workflows are the main mechanism of modularizing functionality wthin scientific workflows.</rdfs:comment>
    </owl:Class>
    


    <!-- http://purl.org/net/wf-motifs#CompositeWorkflow -->

    <owl:Class rdf:about="&motifs;CompositeWorkflow">
        <rdfs:label xml:lang="en">Composite workflow</rdfs:label>
        <rdfs:subClassOf rdf:resource="&motifs;InterWorkflowMotif"/>
        <rdfs:comment xml:lang="en">This motif refers to all those workflows that have one or more sub-workflows included in them (in some cases, these sub-workflows offer different views of the global workflow). </rdfs:comment>
    </owl:Class>
    


    <!-- http://purl.org/net/wf-motifs#ComputationalStep -->

    <owl:Class rdf:about="&motifs;ComputationalStep">
        <rdfs:label xml:lang="en">Computational step</rdfs:label>
        <rdfs:subClassOf rdf:resource="&motifs;IntraWorkflowMotif"/>
        <rdfs:comment>This motif is used to refer to activities that do not require human inputs during their execution.</rdfs:comment>
    </owl:Class>
    


    <!-- http://purl.org/net/wf-motifs#DataAnalysis -->

    <owl:Class rdf:about="&motifs;DataAnalysis">
        <rdfs:label xml:lang="en">Data analysis</rdfs:label>
        <rdfs:subClassOf rdf:resource="http://purl.org/net/wf-motifsl#DataCreation"/>
        <rdfs:comment xml:lang="en">Motif that refers to a broad category of tasks in diverse domains. An important number of workflows are designed with the purpose of analyzing different features of input data, ranging from simple comparisons between the datasets to complex protein analysis to see whether two molecules can be docked successfully or not. </rdfs:comment>
    </owl:Class>
    


    <!-- http://purl.org/net/wf-motifs#DataCleaning -->

    <owl:Class rdf:about="&motifs;DataCleaning">
        <rdfs:label xml:lang="en">Data cleaning</rdfs:label>
        <rdfs:subClassOf rdf:resource="&motifs;OperationMotif"/>
        <rdfs:comment>Steps for cleaning and curating data. Typically these steps are undertaken by sophisticated tooling/services, or by human interactions. A cleaning step essentially preserves and enriches the content of data (e.g., by a user’s annotation of a result with additional information, detecting and removing inconsistencies on the data, etc.).</rdfs:comment>
    </owl:Class>
    


    <!-- http://purl.org/net/wf-motifs#DataMovement -->

    <owl:Class rdf:about="&motifs;DataMovement">
        <rdfs:label xml:lang="en">Data movement</rdfs:label>
        <rdfs:subClassOf rdf:resource="&motifs;OperationMotif"/>
        <rdfs:comment xml:lang="en">Certain analysis activities that are performed via external tools or services require the submission of data to a location accessible by the service/tool (i.e., a web or a local directory respectively). In such cases the workflow contains dedicated step(s) for the upload/transfer of data to these locations. The same applies to the outputs, in which case a data download/retrieval step is used to chain the data to the next steps of the workflow.</rdfs:comment>
    </owl:Class>
    


    <!-- http://purl.org/net/wf-motifs#DataPreparation -->

    <owl:Class rdf:about="&motifs;DataPreparation">
        <rdfs:label xml:lang="en">Data Preparation</rdfs:label>
        <rdfs:subClassOf rdf:resource="&motifs;OperationMotif"/>
        <rdfs:comment xml:lang="en">Data, as it is originally retrieved, may need several transformations before being able to be used in a workflow step. The steps in the workflow performing such transformations can be annotated used the Data Preparation motif.</rdfs:comment>
    </owl:Class>
    


    <!-- http://purl.org/net/wf-motifs#DataRetrieval -->

    <owl:Class rdf:about="&motifs;DataRetrieval">
        <rdfs:label xml:lang="en">Data retrieval</rdfs:label>
        <rdfs:subClassOf rdf:resource="http://purl.org/net/wf-motifsl#DataCreation"/>
        <rdfs:comment>Workflows exploit heterogeneous data sources, remote databases, repositories or other web resources mostly exposed via SOAP or REST services. Scientific data deposited in these repositories are retrieved through query and retrieval steps inside workflows. Certain tasks within the workflow are responsible for retrieving data from such exter- nal source into the workflow environment.</rdfs:comment>
    </owl:Class>
    


    <!-- http://purl.org/net/wf-motifs#DataVisualization -->

    <owl:Class rdf:about="&motifs;DataVisualization">
        <rdfs:label xml:lang="en">Data Visualization</rdfs:label>
        <rdfs:subClassOf rdf:resource="http://purl.org/net/wf-motifsl#DataCreation"/>
        <rdfs:comment xml:lang="en">Being able to show the results is as important as producing them in some workflows. Scientists use visualizations to show the conclusions of their experiments and to take important decisions in the pipeline itself. Therefore certain steps in workflows are dedicated to generation of plots and graph outputs from input data.</rdfs:comment>
    </owl:Class>
    


    <!-- http://purl.org/net/wf-motifs#FormatTransformation -->

    <owl:Class rdf:about="&motifs;FormatTransformation">
        <rdfs:label xml:lang="en">Format transformation</rdfs:label>
        <rdfs:subClassOf rdf:resource="&motifs;UnstructuredDataPreparation"/>
        <rdfs:comment xml:lang="en">Workflows that bring together multiple access or analysis activities usually contain steps for format transformations. Typically, these steps, also known as ”Shims”, preserve the contents of data, while converting its representation format.</rdfs:comment>
    </owl:Class>
    


    <!-- http://purl.org/net/wf-motifs#Group -->

    <owl:Class rdf:about="&motifs;Group">
        <rdfs:label xml:lang="en">Group</rdfs:label>
        <rdfs:subClassOf rdf:resource="&motifs;StructuredDataPreparation"/>
        <rdfs:comment xml:lang="en">Motif that refers to the step or set of steps that reorganize the input into different groups. For example, grouping a table by a certain category.</rdfs:comment>
    </owl:Class>
    


    <!-- http://purl.org/net/wf-motifs#HumanInteraction -->

    <owl:Class rdf:about="&motifs;HumanInteraction">
        <rdfs:label xml:lang="en">Human interaction</rdfs:label>
        <rdfs:subClassOf rdf:resource="&motifs;IntraWorkflowMotif"/>
        <rdfs:comment xml:lang="en">Motif is used to characetrize the activities that require human inputs during their execution.</rdfs:comment>
    </owl:Class>
    


    <!-- http://purl.org/net/wf-motifs#InputAugmentation -->

    <owl:Class rdf:about="&motifs;InputAugmentation">
        <rdfs:label xml:lang="en">Input augmentation</rdfs:label>
        <rdfs:subClassOf rdf:resource="&motifs;UnstructuredDataPreparation"/>
        <rdfs:comment xml:lang="en">Motif that refers to the step or set of steps dedicated to generate aggregation of multiple parameters and scripts for tools and external services.</rdfs:comment>
    </owl:Class>
    


    <!-- http://purl.org/net/wf-motifs#InterWorkflowMotif -->

    <owl:Class rdf:about="&motifs;InterWorkflowMotif">
        <rdfs:label xml:lang="en">Inter-workflow motif</rdfs:label>
        <rdfs:subClassOf rdf:resource="&motifs;WorkflowMotif"/>
        <rdfs:comment xml:lang="en">Motif observed among different workflows.</rdfs:comment>
    </owl:Class>
    


    <!-- http://purl.org/net/wf-motifs#InternalMacro -->

    <owl:Class rdf:about="&motifs;InternalMacro">
        <rdfs:label xml:lang="en">Internal macro</rdfs:label>
        <rdfs:subClassOf rdf:resource="&motifs;IntraWorkflowMotif"/>
        <rdfs:comment xml:lang="en">Motif that refers to those groups of steps in the workflow that correspond to repetitive patterns of combining tasks. </rdfs:comment>
    </owl:Class>
    


    <!-- http://purl.org/net/wf-motifs#IntraWorkflowMotif -->

    <owl:Class rdf:about="&motifs;IntraWorkflowMotif">
        <rdfs:label xml:lang="en">Intra-workflow motif</rdfs:label>
        <rdfs:subClassOf rdf:resource="&motifs;WorkflowMotif"/>
        <rdfs:comment xml:lang="en">Category of motifs observed within a workflow.</rdfs:comment>
    </owl:Class>
    


    <!-- http://purl.org/net/wf-motifs#Join -->

    <owl:Class rdf:about="&motifs;Join">
        <rdfs:label xml:lang="en">Join</rdfs:label>
        <rdfs:subClassOf rdf:resource="&motifs;StructuredDataPreparation"/>
        <rdfs:comment xml:lang="en">Motif that refers to a step or a set of steps that aggregate their contents into a single output. Both intputs generally have the same type</rdfs:comment>
    </owl:Class>
    


    <!-- http://purl.org/net/wf-motifs#Merge -->

    <owl:Class rdf:about="&motifs;Merge">
        <rdfs:label xml:lang="en">Merge</rdfs:label>
        <rdfs:subClassOf rdf:resource="&motifs;UnstructuredDataPreparation"/>
        <rdfs:comment xml:lang="en">Motif that refers to the step of steps in the workflow aggregating information from heterogeneous and unstructured sources</rdfs:comment>
    </owl:Class>
    


    <!-- http://purl.org/net/wf-motifs#Motif -->

    <owl:Class rdf:about="&motifs;Motif">
        <rdfs:label xml:lang="en">Motif</rdfs:label>
        <rdfs:comment xml:lang="en">A motif is a domain independent conceptual abstraction of one or more steps of the workflow</rdfs:comment>
    </owl:Class>
    


    <!-- http://purl.org/net/wf-motifs#OperationMotif -->

    <owl:Class rdf:about="&motifs;OperationMotif">
        <rdfs:label xml:lang="en">Operation motif</rdfs:label>
        <rdfs:subClassOf rdf:resource="&motifs;Motif"/>
        <rdfs:comment xml:lang="en">An operation motif describes the data manipulation and/or transformation carried out by a step in the workflow, a collection of steps in the workflow or a subworkflow</rdfs:comment>
    </owl:Class>
    


    <!-- http://purl.org/net/wf-motifs#OutputExtraction -->

    <owl:Class rdf:about="&motifs;OutputExtraction">
        <rdfs:label xml:lang="en">Output extraction</rdfs:label>
        <rdfs:subClassOf rdf:resource="&motifs;UnstructuredDataPreparation"/>
        <rdfs:comment xml:lang="en">Motif that refers to the step or set of steps in the workflow that retrieve only the relevant portion from the the output of a previous step. For example, retrieving the tag value of an XML fragment.</rdfs:comment>
    </owl:Class>
    


    <!-- http://purl.org/net/wf-motifs#Sort -->

    <owl:Class rdf:about="&motifs;Sort">
        <rdfs:label xml:lang="en">Sort</rdfs:label>
        <rdfs:subClassOf rdf:resource="&motifs;StructuredDataPreparation"/>
        <rdfs:comment xml:lang="en">Motif that refers to the step or set of steps ordering the input by certain parameter. For example, a quicksort algorithm that takes an unorderd vector and produces a sorted output.</rdfs:comment>
    </owl:Class>
    


    <!-- http://purl.org/net/wf-motifs#StructuredDataPreparation -->

    <owl:Class rdf:about="&motifs;StructuredDataPreparation">
        <rdfs:label xml:lang="en">Structured data preparation</rdfs:label>
        <rdfs:subClassOf rdf:resource="&motifs;DataPreparation"/>
        <rdfs:comment xml:lang="en">Data preparation motifs that require the some of all of the inputs to be structured in tables, excel files, etc.</rdfs:comment>
    </owl:Class>
    


    <!-- http://purl.org/net/wf-motifs#SynchronousInvocaton -->

    <owl:Class rdf:about="&motifs;SynchronousInvocaton">
        <rdfs:label xml:lang="en">Synchronous invocation</rdfs:label>
        <rdfs:subClassOf rdf:resource="&motifs;IntraWorkflowMotif"/>
        <rdfs:comment xml:lang="en">Motif that requires a single step for performing a service call or tool invocation.</rdfs:comment>
    </owl:Class>
    


    <!-- http://purl.org/net/wf-motifs#UnstructuredDataPreparation -->

    <owl:Class rdf:about="&motifs;UnstructuredDataPreparation">
        <rdfs:label xml:lang="en">Unstructured data preparation</rdfs:label>
        <rdfs:subClassOf rdf:resource="&motifs;DataPreparation"/>
        <rdfs:comment xml:lang="en">Data preparation motifs that don&apos;t require some of all of the inputs to be structured in tables, excel files, etc.</rdfs:comment>
    </owl:Class>
    


    <!-- http://purl.org/net/wf-motifs#WorkflowMotif -->

    <owl:Class rdf:about="&motifs;WorkflowMotif">
        <rdfs:subClassOf rdf:resource="&motifs;Motif"/>
        <rdfs:comment xml:lang="en">A workflow motif describes how an operation motif is realized (i.e., implemented) within a workflow.</rdfs:comment>
        <rdfs:comment xml:lang="en">Workflow motif</rdfs:comment>
    </owl:Class>
    


    <!-- http://purl.org/net/wf-motifs#WorkflowOverload -->

    <owl:Class rdf:about="&motifs;WorkflowOverload">
        <rdfs:label xml:lang="en">Workflow overload</rdfs:label>
        <rdfs:subClassOf rdf:resource="&motifs;InterWorkflowMotif"/>
        <rdfs:comment xml:lang="en">Motif used to characetrize workflows that are used to operate over different input parameter types. An example is performing an analysis over a String input parameter, or performing it over the contents of a specified File. Overloading is a direct response to the heterogeneity of environments in which workflows are used.</rdfs:comment>
    </owl:Class>
    


    <!-- http://purl.org/net/wf-motifsl#DataCreation -->

    <owl:Class rdf:about="http://purl.org/net/wf-motifsl#DataCreation">
        <rdfs:label xml:lang="en">Data creation</rdfs:label>
        <rdfs:subClassOf rdf:resource="&motifs;OperationMotif"/>
        <rdfs:comment xml:lang="en">Motif that represents a step or set of steps where new data is created by the workflow. It serves to highlight the main functionality of the workflow.</rdfs:comment>
    </owl:Class>
    


    <!-- http://purl.org/net/wf-motifsl#Filter -->

    <owl:Class rdf:about="http://purl.org/net/wf-motifsl#Filter">
        <rdfs:label xml:lang="en">Filter
</rdfs:label>
        <rdfs:subClassOf rdf:resource="&motifs;StructuredDataPreparation"/>
        <rdfs:comment xml:lang="en">Motif that refers to a filtering step or set of steps. For example, A file filtered by a set of set of keywords, a table filtered by a threshold, etc.</rdfs:comment>
    </owl:Class>
    


    <!-- http://purl.org/net/wf-motifsl#Split -->

    <owl:Class rdf:about="http://purl.org/net/wf-motifsl#Split">
        <rdfs:label xml:lang="en">Split</rdfs:label>
        <rdfs:subClassOf rdf:resource="&motifs;UnstructuredDataPreparation"/>
        <rdfs:comment xml:lang="en">Motif that refers to the step or steps in the workflow that separate an input into different outputs.</rdfs:comment>
    </owl:Class>
</rdf:RDF>



<!-- Generated by the OWL API (version 3.3.1957) http://owlapi.sourceforge.net -->

